remove unnnecessary curry notation

Cm/Pi/Curry.lean
@@ -6,103 +6,102 @@ import Cm.Pi.Util
 open Expr
 
 /-
-Thought:
-- partial apply? We have partial both. Why not both?
+Utility methods for currying that simulate lambda calculus binders with de bruijn indices.
+In the list calculus, arguments are usually positional, not curried.
+This gets around that by growing the context in a sequence, cons'ing each argument as it is applied.
+
+The three main operators are:
+args.read, args.push, $args, and lam.
+var.read `n` creates a (:: π (:: nil (:: π ... id))) expression with `n` nil entries.
+This skips the first `n` elements in a context and gets the last one.
+
+args.push pushes an argument to the arguments list of a function.
+args.store expects that the context / arguments list is in scope.
+
+(:: apply (:: (:: apply (:: args.push x)) args)) = (:: x args)
+args.push = (:: both (:: (quote both) (:: both
+  const
+  (quote id))))
+
+$args spreads the context / arguments list among many operations,
+and applies the args to each function.
+
+(:: apply (:: (:: apply (:: $args (:: f (:: g h)))) args)) =
+(:: (:: apply (:: f args)) (:: (:: apply (:: g args)) (:: apply h args)))
+
+(:: apply (:: lam body)) creates a (:: both (:: (quote body) args.store)) expression.
+This is essentially one level of currying.
+Applying other arugments will just push this argument to the front of them.
+
+(:: apply (:: (:: apply (:: (:: apply (:: lam body)) (symbol "arg"))) other_args))
+= (:: apply (:: body (:: (symbol "arg") other_args)))
+
+TODO:
+- these old utility methods may not actually work as intended.
 -/
 
-/-
-Expects the first both argument, but will wait for the second.
+def mk_π_skip (n : ℕ) (at_end : Expr) : Expr :=
+  match n with
+  | .zero => :: π (:: at_end nil)
+  | n => (List.replicate n nil).foldr (fun e acc => (:: π (:: e acc))) (:: π (:: at_end nil))
 
-(:: (:: both_partial f) x) = (:: f x)
--/
-def both_partial : Expr :=
-  (:: both (:: (quote both) (:: both (:: const (quote id)))))
+example : mk_π_skip 2 id = (:: π (:: nil (:: π (:: nil (:: π (:: id nil)))))) := rfl
 
-def test_both_partial : Except Error Expr := do
-  let my_f := symbol "f"
-  let my_x := symbol "x"
+def args.read (n : ℕ) (e : Expr) : Expr := mk_π_skip n e
 
-  do_step (:: apply (:: (:: apply (:: both_partial my_f)) my_x))
+example : try_step_n' 5 (:: apply (:: (args.read 0 id) (:: (symbol "a") nil))) = (.ok (symbol "a")) := rfl
+example : try_step_n' 5 (:: apply (:: (args.read 2 id) (:: (symbol "a") (:: (symbol "b") (:: (symbol "c") nil))))) = (.ok (symbol "c")) := rfl
+example : try_step_n' 5 (:: apply (:: (args.read 0 id) (:: (symbol "a") (:: (symbol "b") (symbol "c"))))) = (.ok (symbol "a")) := rfl
 
--- :: "f" "x"
-#eval test_both_partial
+def args.push : Expr := (:: both (::
+  (quote both) (:: both (::
+    const
+    (quote id)))))
 
-/-
-:: apply (:: f x) = (:: (:: apply_partial f) x)
--/
-def apply_partial : Expr :=
-  (:: both (:: (quote both) (:: both (:: (quote (quote apply)) (:: both (:: (quote both) (:: both (:: const (quote id)))))))))
+example : try_step_n' 5
+  (:: apply
+    (:: (:: apply (:: args.push (symbol "arg"))) (:: (symbol "args") nil))) =
+    (.ok (:: (symbol "arg") (:: (symbol "args") nil))) := rfl
 
-def test_apply_partial : Except Error Expr := do
-  let my_f := symbol "f"
-  let my_x := symbol "x"
+example : try_step_n' 5 (:: apply (:: (:: apply (:: args.push (symbol "arg"))) nil)) =
+  (.ok (:: (symbol "arg") nil)) := rfl
 
-  do_step (:: apply (:: (:: apply (:: apply_partial my_f)) my_x))
+def args.app (e : Expr) :=
+  match e with
+  | :: x nil => (:: both (:: (:: both (:: (quote apply) (:: both (:: (quote x) id)))) (quote nil)))
+  | :: x xs => (:: both (::
+    (:: both (:: (quote apply) (:: both (:: (quote x) id))))
+    (args.app xs)))
+  | e => (quote e)
 
-/-def test_apply_partial' : Except Error Expr := do
-  -- this will only work with an :: x xs argument
-  let my_f := π id id
-  let -/
+def args.app.test_args : Expr := (:: (symbol "a") (:: (symbol "b") (:: (symbol "c") nil)))
+def args.app.test_ops : Expr := (:: (args.read 0 id) (:: (args.read 1 id) (:: (args.read 2 id) nil)))
 
--- :: "f" "x"
-#eval test_apply_partial
+example : try_step_n' 10 (:: apply (:: (args.app args.app.test_ops) args.app.test_args)) = (.ok args.app.test_args) := rfl
 
-/-
-curry = apply_partial?
+def curry.push_future_arg := (quote (:: both (:: (quote apply) (:: both (:: (quote args.push) id)))))
 
-apply_partial only works for one argument, which is confusing.
-:: apply technically works for n-ary arguments.
-More like one single massive array argument.
+def curry : Expr := (:: both (:: (quote both)
+    (:: both (:: (quote (quote both)) (:: both (:: (quote both)
+      (:: both (:: (quote (quote (quote apply))) (:: both (:: (quote both)
+        (:: both (:: (quote (quote both)) (:: both (:: (quote both)
+          (:: both (:: (:: both (:: (quote const) const)) curry.push_future_arg))))))))))))))))
 
-Note: x is parametric in full in apply_partial, meaning
-x itself could be derived partially, perhaps with both_partial.
+example : try_step_n' 50 (:: apply (:: (:: apply (:: (:: apply (:: curry.push_future_arg (args.app (:: (quote (symbol "arg: ")) (:: (args.read 0 id) nil))))) (symbol "hi"))) (:: (symbol "other arg") (:: (symbol "other other arg") nil))))
+  = (.ok (:: (symbol "hi") (:: (symbol "other arg") (:: (symbol "other other arg") nil)))) := rfl
 
-Example using apply_partial:
+set_option maxRecDepth 1000
 
-(:: (:: apply_partial f) (:: (:: both_partial x) xs))
-  = (:: f (:: x xs))
+example : try_step_n' 100 (:: apply (::
+  (:: apply (:: (:: apply (:: curry
+    (args.app (:: (quote (symbol "ctx: ")) (:: id nil)))))
+    (symbol "hi")))
+    (:: (symbol "other arg") (:: (symbol "other other arg") nil)))) =
+  (.ok (:: (symbol "ctx: ") (:: (:: (symbol "hi")
+    (:: (symbol "other arg") (:: (symbol "other other arg") nil)))
+    nil))) := rfl
 
-apply_partial probably won't let us easily pipeline the way we want,
-but we can pipeline the both right half.
--/
+example : try_step_n' 100 (:: apply (:: (:: apply (:: (:: apply (:: curry (args.read 0 id))) (symbol "arg 0"))) (symbol "rest args")))
+   = (.ok (symbol "arg 0")) := rfl
 
-/-
-The same example as above, except my_x is partially applied
--/
-def test_apply_partial' : Except Error Expr := do
-  let my_f := Expr.id
-  let my_x := symbol "x"
-
-  do_step (:: apply (:: (:: apply (:: apply_partial my_f)) my_x))
-
-#eval test_apply_partial'
-
-/-
-The original test, not partially applied.
--/
-def test_apply_partial'' : Except Error Bool := do
-  let my_f := (:: π (:: id (:: π (:: id (:: const nil)))))
-  let my_arg := (:: (symbol "a") (:: (symbol "b") (:: (symbol "c") nil)))
-  let expected ←  do_step (:: apply (:: my_f my_arg))
-  let actual ← do_step (:: apply (:: (:: apply (:: apply_partial my_f)) my_arg))
-  pure <| actual == expected
-
-#eval test_apply_partial''
-
---def curry : Expr :=
-  
-
-
-/-
-Simple case: currying once.
-(X × Y) → Z => X → (Y → Z)
-
-This is just both_partial.
--/
-
-/-
-curr 0 f = nil
-curr 1 f = 
--/
-/-def curr : ℕ → Expr
-  | .zero => id-/
+example : try_step_n' 51 (:: apply (:: (:: apply (:: (:: apply (:: (:: apply (:: curry (:: apply (:: curry (args.read 1 id))))) (symbol "arg 0"))) (symbol "rest args"))) (:: (symbol ("other arg")) nil))) = (.ok (symbol "other arg")) := rfl
